BDD/Basic.lean
@@ -1,40 +1,21 @@
 import Std
 import Common.DDClasses
 
-inductive BDD where
-  | leaf (id' : Nat) (value : Bool)
-  | node (id' : Nat) (left right : BDD)
-deriving BEq, Hashable, Repr
+structure BDD where
+  tree : Node
+  unusedId : Nat := 2
+deriving BEq
 
-instance : Inhabited BDD where
-  default := .leaf 0 false
+def BDD.addNewConstant (self: BDD) (_value : Bool) : BDD :=
+  self
 
-def BDD.id (self : BDD) : Nat := match self with
-  | .leaf id' _ => id'
-  | .node id' _ _ => id'
+def BDD.addNewVar (self: BDD) (_index : Nat) (_low _high : Node) : BDD :=
+  self
 
-def BDD.low (self : BDD) : Option BDD := match self with
-  | .leaf _ _ => none
-  | .node _ left _ => some left
-
-def BDD.high (self : BDD) : Option BDD := match self with
-  | .leaf _ _ => none
-  | .node _ _ right => some right
-
-instance : DecisionDiagramTree BDD where
-  id := BDD.id
---  newConstant : Bool → BDD := sorry
---  addNewVar (index: Nat) (low high : BDD) : BDD := sorry
---  isConstant : BDD → Bool := sorry
---  unifiedKey : BDD → Nat := sorry
---  index : BDD → Option Nat := sorry
-  low := BDD.low
-  high := BDD.high
+instance : DecisionDiagram BDD where
+  allNodes (self : BDD) := Node.toHashSet self.tree
+  addNewConstant := BDD.addNewConstant
+  addNewVar (self : BDD) (index : Nat) (low high : Node) := self.addNewVar index low high
 --  buildIndexer : BDD → Std.HashMap BDD Nat × Std.HashMap Nat BDD := sorry
 
-example : (default : BDD).id = 0 := rfl
-
-instance : ToString BDD where
-  toString := fun bdd => match bdd with
-    | .leaf id' value => s!"leaf {id'} {value}"
-    | .node id' left right => s!"node {id'} {left.id} {right.id}"
+example : (default : Node).index = 0 := rfl
